garbage

btree.dfy
@@ -46,36 +46,253 @@ lemma lexical_cmp_between_implies_common_prefix(a: string, b: string, c: string)
 	}
 }
 
+///////////////////////////////////////////
 
+function method seq_map<U,T>(f: T-> U, inputs: seq<T>) : seq<U>
+	decreases inputs;
+{
+	if |inputs| == 0 then []
+	else [f(inputs[0])] + seq_map(f, inputs[1..])
+}
 
-// datatype Node<Key, Value> =
-// 	Leaf(keys: array<Key>, values: array<Value>) |
-// 	Index(pivots: array<int>, children: array<Node>)
+function method seq_fold_left<U,T>(f: (U, T) -> U, acc: U, inputs: seq<T>) : U
+{
+	if |inputs| == 0 then acc
+	else seq_fold_left(f, f(acc, inputs[0]), inputs[1..])
+}
 
-// datatype BtreeConfig<!Key, Value> = BtreeConfig(
+datatype Node =
+	Leaf(keys: seq<string>, values: seq<int>) |
+	Index(pivots: seq<string>, children: seq<Node>)
+
+// function num_nodes(node: Node) : int
+// {
+// 	match node {
+// 		case Leaf(keys, values) => 1
+// 		case Index(pivots, children) =>
+			
+// 	}
+// }
+
+function method set_of_keys_of_children(nodes: seq<Node>, ghost height: int, ghost max_fanout: int) : set<string>
+	decreases height * max_fanout;
+{
+	if |nodes| == 0 then {}
+	else set_of_keys(nodes[0], m-1) + set_of_keys_of_children(nodes[1..], m)
+}
+
+function method set_of_keys(node: Node, ghost m: int) : set<string>
+	requires m == num_nodes(node);
+	//requires subtree_is_well_formed(node);
+	//decreases node;
+	decreases m;
+{	
+	match node {
+		case Leaf(keys, values) =>
+			set k | k in multiset(keys)
+		case Index(pivots, children) =>
+			children_have_lower_max_height(node);
+			//seq_fold_left((a, b) => a + b, {}, seq_map(x => set_of_keys(x), children))
+			set_of_keys_of_children(children, m-1)
+	}
+}
+
+// predicate subtree_is_well_formed(node: Node) {
+// 	match node {
+// 		case Leaf(keys, values) =>
+// 			|keys| > 0 &&
+// 			|keys| == |values|
+// 		case Index(pivots, children) =>
+// 			|pivots| > 0 &&
+// 			|pivots| == |children| - 1 &&
+// 			forall i :: 0 <= i < |children| ==> subtree_is_well_formed(children[i])
+// 	}
+// }
+
+// predicate seq_is_strictly_increasing(ss: seq<string>) {
+// 	forall i :: 0 <= i < |ss|-1 ==> lexical_cmp(ss[i], ss[i+1]) < 0
+// }		
+
+// predicate subtree_is_sorted(node: Node)
+// 	requires subtree_is_well_formed(node);
+// {
+// 	match node {
+// 		case Leaf(keys, values) =>
+// 			seq_is_strictly_increasing(keys)
+// 		case Index(pivots, children) =>
+// 			seq_is_strictly_increasing(pivots) &&
+// 			(forall i :: 0 <= i < |children|-1 ==>
+// 			  (forall x :: x in set_of_keys(children[i]) ==>
+// 			    lexical_cmp(x, pivots[i]) < 0)) &&
+// 			(forall i :: 1 <= i < |children| ==>
+// 			  (forall x :: x in set_of_keys(children[i]) ==>
+// 			    lexical_cmp(pivots[i-1], x) <= 0)) &&
+// 			forall i :: 0 <= i < |children| ==> subtree_is_sorted(children[i])
+// 	}
+// }
+
+// function map_of_kvpairs(acc: map<string, int>, keys: seq<string>, values: seq<int>) : map<string, int>
+// 	requires |keys| == |values|;
+// {
+// 	if |keys| == 0 then acc
+// 	else map_of_kvpairs(acc, keys[1..], values[1..])[keys[0] := values[0]]
+// }
+
+// function map_of_children(acc: map<string, int>, nodes: seq<Node>) : map<string, int>
+// 	requires forall i :: 0 <= i < |nodes| ==> subtree_is_well_formed(nodes[i]);
+// 	requires forall i :: 0 <= i < |nodes| ==> subtree_is_sorted(nodes[i]);
+// {
+// 	if |nodes| == 0 then acc
+// 	else map_of_children(map_of_subtree(acc, nodes[0]), nodes[1..])
+// }
+
+// function map_of_subtree(acc: map<string, int>, node: Node) : map<string, int>
+// 	requires subtree_is_well_formed(node);
+// 	requires subtree_is_sorted(node);
+// {
+// 	match node {
+// 		case Leaf(keys, values) =>
+// 			map_of_kvpairs(acc, keys, values)
+// 		case Index(pivots, children) =>
+// 			max_height_is_nonnegative(node);
+// 			assert forall i :: 0 <= i < |children| ==> max_height(children[i]) < max_height(node);
+// 			map_of_children(acc, children)
+// 	}
+// }
+
+// function subtree_map_contents(node: Node) : map<string, int>
+// 	requires subtree_is_well_formed(node);
+// 	requires subtree_is_sorted(node);
+// {
+// 	map_of_subtree(map[], node)
+// }
+
+// function method min(a: int, b: int) : int
+// {
+// 	if a < b
+// 		then a
+// 	else
+// 		b
+// }
+
+function method max(a: int, b: int) : int
+{
+	if a < b
+		then b
+	else
+		a
+}
+
+// function min_height_of_children(nodes: seq<Node>) : int
+// 	requires forall i :: 0 <= i < |nodes| ==> subtree_is_well_formed(nodes[i]);
+// 	requires |nodes| > 0;
+// {
+// 	if |nodes| == 1 then min_height(nodes[0])
+// 	else min(min_height(nodes[0]), min_height_of_children(nodes[1..]))
+// }
+
+// function min_height(node: Node) : int
+// 	requires subtree_is_well_formed(node);
+// {
+// 	match node {
+// 		case Leaf(keys, values) => 0
+// 		case Index(pivots, children) => 1 + min_height_of_children(children)
+// 	}
+// }
+
+function max_height_of_children(nodes: seq<Node>) : int
+	//requires forall i :: 0 <= i < |nodes| ==> subtree_is_well_formed(nodes[i]);
+	//requires |nodes| > 0;
+	ensures max_height_of_children(nodes) >= 0;
+	ensures forall i :: 0 <= i < |nodes| ==> max_height(nodes[i]) <= max_height_of_children(nodes);
+{
+	if |nodes| == 0 then 0
+	else if |nodes| == 1 then max_height(nodes[0])
+	else max(max_height(nodes[0]), max_height_of_children(nodes[1..]))
+}
+
+function max_height(node: Node) : int
+	//requires subtree_is_well_formed(node);
+	ensures max_height(node) >= 0;
+{
+	match node {
+		case Leaf(keys, values) => 0
+		case Index(pivots, children) => 1 + max_height_of_children(children)
+	}
+}
+
+lemma max_height_is_nonnegative(node: Node)
+	//requires subtree_is_well_formed(node);
+	ensures max_height(node) >= 0;
+{
+}
+
+lemma children_have_lower_max_height(node: Node)
+	requires node.Index?;
+	ensures forall i :: 0 <= i < |node.children| ==> max_height(node.children[i]) == max_height(node) - 1;
+{
+	assume false;
+	if |node.children| > 0 {
+		assert max_height(node.children[0]) == max_height(node) - 1;
+	}
+}
+
+// predicate subtree_is_balanced(node: Node)
+// 	requires subtree_is_well_formed(node);
+// {
+// 	min_height(node) == max_height(node)
+// }
+
+// datatype Config = Config(
 // 	min_leaf_size: int, max_leaf_size: int,
-//   min_fanout: int, max_fanout: int,
-// 	comparator: (Key, Key) -> int)
+//   min_fanout: int, max_fanout: int)
 
-// predicate is_total_order<Key>(cmp: (int, int) -> int) {
-//  	forall a: int :: forall b: int :: cmp(a,b) < 0 <==> cmp(b, a) > 0
+// predicate well_formed_config(cfg: Config) {
+// 	1 <= cfg.min_leaf_size < cfg.max_leaf_size &&
+// 	2 <= cfg.min_fanout < cfg.max_fanout
+// }
+
+// predicate subtree_satisfies_config(node: Node, cfg: Config) {
+// 	match node {
+// 		case Leaf(keys, pivots) =>
+// 			cfg.min_leaf_size <= |keys| <= cfg.max_leaf_size
+// 		case Index(pivots, children) =>
+// 			cfg.min_fanout <= |children| < cfg.max_fanout &&
+// 			forall i :: 0 <= i < |children| ==> subtree_satisfies_config(children[i], cfg)
+// 	}
+// }
+
+// predicate is_valid_b_subtree(node: Node, cfg: Config) {
+// 	subtree_is_well_formed(node) &&
+// 		subtree_is_sorted(node) &&
+// 		subtree_is_balanced(node) &&
+// 		subtree_satisfies_config(node, cfg)
+// }
+
+// datatype QueryResult = KeyDoesNotExist | Value(v: int)
+
+// function method search_seq(keys: seq<string>, values: seq<int>, key: string) : QueryResult
+// 	requires seq_is_strictly_increasing(keys);
+// 	requires |keys| == |values|;
+// 	ensures key !in map_of_kvpairs(map[], keys, values) ==>
+// 		search_seq(keys, values, key) == KeyDoesNotExist;
+// 	ensures key in map_of_kvpairs(map[], keys, values) ==>
+// 		search_seq(keys, values, key) == Value(map_of_kvpairs(map[], keys, values)[key]);
+// {
+// 	if |keys| == 0 then KeyDoesNotExist
+// 	else if keys[0] == key then Value(values[0])
+// 	else search_seq(keys[1..], values[1..], key)
 // }
 	
-// // predicate valid_btree_config<Key, Value>(cfg: BtreeConfig<Key, Value>) {
-// // 	1 <= cfg.min_leaf_size &&
-// // 		  cfg.min_leaf_size < cfg.max_leaf_size &&
-// // 	2 <= cfg.min_fanout &&
-// // 	    cfg.min_fanout < cfg.max_fanout &&
-// // 	forall a: Key :: forall b: Key :: cfg.comparator(a,b) < 0 <==> cfg.comparator(b, a) > 0 &&
-// // 	forall a: Key :: forall b: Key :: cfg.comparator(a,b) == 0 <==> cfg.comparator(b, a) == 0 &&
-// // 	forall a: Key :: forall b: Key :: forall c: Key :: cfg.comparator(a, b) < 0 && cfg.comparator(b, c) < 0 ==> cfg.comparator(a, c) < 0
+// // function method query(node: Node, key: string) : QueryResult
+// // 	requires subtree_is_well_formed(node);
+// // 	requires subtree_is_sorted(node);
+// // 	ensures key !in subtree_map_contents(node) <==> query(node, key) == KeyDoesNotExist;
+// // 	ensures key in subtree_map_contents(node) <==> query(node, key) == Value(subtree_map_contents(node)[key]);
+// // {
+// // 	match node {
+// // 		case Leaf(keys, values) =>
+			
+// // 		case Index(pivots, children) =>
+// // 	}
 // // }
-
-// function method int_compare(a: int, b: int) : int {
-// 	a - b
-// }
-
-// method dummy(x: int) returns (nada: int) {
-// 	var cfg: BtreeConfig<int, int> := BtreeConfig(12, 24, 80, 160, int_compare);
-// 	nada := 0;
-// }
